progress

src/examples/implang_cont_eg.v
@@ -8,7 +8,7 @@ Local Open Scope func_scope.
 Definition min_positive :=
   fn "l" <{ ( "min" "v" )
     "min" <a- #0 ;;
-    While !"l" ≠ #0 <{
+    While "l" ≠ #0 <{
       (* If !"l" < !"min" <{ break }> ;; *)
       "v" <a- !"l";;
       "l" <a- !("l" + #1);;
@@ -34,11 +34,12 @@ Section spec.
     (l + i)%Z.
   Notation "l +ₗ i" := (ptr_add l i) (at level 10, left associativity).
 
-  (* a linked list starting with l and stores lv; tail pointer is `last` *)
+  (* a segment of linked list starting with l and stores lv;
+    the last cell has pointer `last` that might or might not be empty *)
   Fixpoint llist_seg (l: loc) (lv: list Z) (last: loc) : assert :=
     match lv with
     | [] => ⌜l = last⌝
-    | v :: lv' => ∃ l', l ↦ NumV v ∗ (l+ₗ1) ↦ LocV l' ∗ llist_seg l' lv' last
+    | v :: lv' => ⌜l≠0%Z⌝ ∧ ∃ l', l ↦ NumV v ∗ (l+ₗ1) ↦ LocV l' ∗ llist_seg l' lv' last
     end.
 
   Definition llist (l: loc) (lv: list Z) := llist_seg l lv 0%Z.
@@ -69,22 +70,44 @@ Section spec.
   (* ad-hoc, aggressive *)
   Ltac iSteps := repeat first [iStep | iModIntro | progress iFrame | progress iIntros ].
 
-  Lemma min_positive_spec E (l: loc) (lv: list Z) z :
+  Lemma min_positive_spec E (l: loc) (lv: list Z) :
     (∃ _z, "r" ↦v NumV _z) ∗ l ↦ₗ lv
-    ⊢ call_assert F E min_positive [LocV l; NumV 0; NumV 0] "r" ("r" ↦v NumV z ∗ l ↦ₗ lv ∗ ⌜min_positive_r lv = z⌝).
+    ⊢ call_assert F E min_positive [LocV l; NumV 0; NumV 0] "r" ("r" ↦v NumV (min_positive_r lv) ∗ l ↦ₗ lv).
   Proof.
     iIntros "((%_z & r) & arr)".
     wp_start_func with_retainer "retainer" and_locals "(l & min & v & _)".
     iSteps.
     simpl.
 
-    set (∃ l_m lv_a lv_b, ⌜lv = lv_a++lv_b⌝ ∧ l ↦ₛ lv_a l_m ∗ l_m ↦ₗ lv_b ∗
-                "l" ↦v (LocV l_m) ∗ "v" ↦v (NumV (min_positive_r lv_a)))%I%Z as inv.
-    wp_apply (wp_while_inv  _ _ _ _ inv with "[] [-r retainer]" ) ; simpl.
+    set (∃ l_m lv_a lv_b v, ⌜lv = lv_a++lv_b ⌝ ∧ l ↦ₛ lv_a l_m ∗ l_m ↦ₗ lv_b ∗
+                "l" ↦v (LocV l_m) ∗ "v" ↦v v ∗ "min" ↦v (NumV (min_positive_r lv_a)) ∗
+                stack_retainer min_positive ∗ (∃ _z, ⇓ ("r" ↦v _z)))%I%Z as inv.
+    wp_apply (wp_while_inv  _ _ _ _ inv with "[] [-]" ) ; simpl.
     {
-      iIntros "!> (%l_m & %lv_a & %lv_b & %Hlv & arr_a & arr_b & l & v)".
-      { iSteps. 
-      
+      iIntros "!> (%l_m & %lv_a & %lv_b & %v & -> & arr_a & arr_b & l & v & min & retainer & (%_z' & r))".
+      iSteps.
+      destruct (bool_decide (l_m = 0%Z)) eqn: Heqb; rewrite Heqb;
+        [rewrite bool_decide_eq_true in Heqb; subst | rewrite bool_decide_eq_false in Heqb].
+      - iExists _. iSplit; first done.
+        iSteps.
+        iSplitL "l v min".
+        { iExists [_;_;_]. iSplit; first done. by iFrame. }
+        iIntros "!> !> r". iFrame.
+        destruct lv_b. 2: { rewrite /llist {2}/llist_seg /=. iDestruct "arr_b" as "[% ?]". done. }
+        rewrite app_nil_r. iFrame.
+      - iExists _. iSplit; first done.
+        iSteps. simpl.
+        iSteps.
+        admit.
+    }
+    {
+      rewrite /inv. iFrame. iExists []. rewrite app_nil_l /=. by iFrame.
+    }
+    iSteps.
+    iRename select (_) into "inv".
+    iDestruct "inv" as "(%l_m & %lv_a & %lv_b & %v & -> & arr_a & arr_b & l & v & min & retainer & (%_z' & r))".
+    (* TODO need to show l_m=0 or lv_b=[] *)
+    iSteps.
   Admitted.
 
 End spec.
